current-formalism/Gathering/InR2/Peleg.v
@@ -1,0 +1,1358 @@
+(**************************************************************************)
+(**   Mechanised Framework for Local Interactions & Distributed Algorithms 
+
+   T. Balabonski, P. Courtieu, L. Rieg, X. Urbain                            
+
+   PACTOLE project                                                      
+                                                                        
+   This file is distributed under the terms of the CeCILL-C licence     
+                                                                        *)
+(**************************************************************************)
+
+
+Set Automatic Coercions Import. (* coercions are available as soon as functor application *)
+Require Import Bool.
+Require Import Arith.Div2.
+Require Import Omega Field.
+Require Import Rbase Rbasic_fun R_sqrt Rtrigo_def.
+Require Import List.
+Require Import SetoidList.
+Require Import Relations.
+Require Import RelationPairs.
+Require Import Morphisms.
+Require Import Psatz.
+Require Import Inverse_Image.
+Require Import Pactole.Preliminary.
+Require Import Pactole.Robots.
+Require Import Pactole.Configurations.
+Require Pactole.CommonFormalism.
+Require Pactole.FlexibleFormalism.
+Require Import Pactole.MultisetSpectrum.
+Require Import Pactole.Lexprod.
+Require Import Pactole.Gathering.InR2.R2geometry.
+Require Import Pactole.Gathering.FlexDefinitionsMultiset.
+
+
+Import Permutation.
+Set Implicit Arguments.
+
+
+(** *  The Gathering Problem  **)
+
+(** Vocabulary: we call a [location] the coordinate of a robot.
+    We call a [configuration] a function from robots to configuration.
+    An [execution] is an infinite (coinductive) stream of [configuration]s.
+    A [demon] is an infinite stream of [demonic_action]s. *)
+
+Module GatheringinR2.
+
+(** **  Framework of the correctness proof: a finite set with at least two elements  **)
+
+Parameter nG: nat.
+Axiom Hyp_nG : (2 <= nG)%nat.
+
+(** There are nG good robots and no byzantine ones. *)
+Module N : Size with Definition nG := nG with Definition nB := 0%nat.
+  Definition nG := nG.
+  Definition nB := 0%nat.
+End N.
+
+(** We instantiate in our setting the generic definitions of the gathering problem. *)
+Module Defs := FlexDefinitionsMultiset.FlexGatheringDefs(R2)(N).
+Import Defs.
+
+Lemma no_byz : forall (id : Names.ident) P, (forall g, P (Good g)) -> P id.
+Proof.
+intros [g | b] P HP.
++ apply HP.
++ destruct b. unfold N.nB in *. omega.
+Qed.
+
+Lemma no_byz_eq : forall config1 config2 : Config.t,
+  (forall g, R2.eq (Config.loc (config1 (Good g))) (Config.loc (config2 (Good g)))) -> Config.eq config1 config2.
+Proof. intros config1 config2 Heq id. apply no_info, (no_byz id). intro g. apply Heq. Qed.
+
+Lemma Config_list_alls : forall pt, Config.list (fun _ => pt) = alls pt N.nG.
+Proof.
+intro. rewrite Config.list_spec, map_cst.
+setoid_rewrite Names.names_length. unfold N.nB. now rewrite plus_0_r.
+Qed.
+
+Definition Spect_map f s := Spect.M.fold (fun e acc => Spect.M.add (f e) acc) s Spect.M.empty.
+
+Lemma map_sim_support : forall (sim : Sim.t) s,
+  Permutation (Spect.M.support (Spect_map sim s)) (map sim (Spect.M.support s)).
+Proof.
+intros sim s. rewrite <- PermutationA_Leibniz. apply Spect.map_injective_support.
+- intros ? ? Heq. now rewrite Heq.
+- apply Sim.injective.
+Qed.
+
+Lemma map_sim_elements : forall (sim : Sim.t) s,
+  PermutationA Spect.Mraw.eq_pair (Spect.M.elements (Spect_map sim s))
+              (map (fun xn => (sim (fst xn), snd xn)) (Spect.M.elements s)).
+Proof.
+intros sim s. apply Spect.map_injective_elements.
+- intros ? ? Heq. now rewrite Heq.
+- apply Sim.injective.
+Qed.
+
+(** Spectra can never be empty as the number of robots is non null. *)
+Lemma spect_non_nil : forall conf, ~Spect.eq (!! conf) Spect.M.empty.
+Proof. apply spect_non_nil. assert (Hle := Hyp_nG). unfold N.nG. omega. Qed.
+
+Lemma support_non_nil : forall config, Spect.M.support (!! config) <> nil.
+Proof.
+intros config Habs.
+rewrite Spect.M.support_nil in Habs.
+apply (spect_non_nil _ Habs).
+Qed.
+
+Lemma gathered_at_dec : forall config pt, {gathered_at pt config} + {~gathered_at pt config}.
+Proof.
+intros config pt.
+destruct (forallb (fun id => R2dec_bool (config id) pt) Names.names) eqn:Hall.
++ left. rewrite forallb_forall in Hall. intro g. rewrite <- R2dec_bool_true_iff. apply Hall, Names.In_names.
++ right. rewrite <- negb_true_iff, existsb_forallb, existsb_exists in Hall. destruct Hall as [id [Hin Heq]].
+  revert Hin Heq. apply (no_byz id). clear id. intros g Hin Heq Habs. specialize (Habs g).
+  rewrite negb_true_iff, R2dec_bool_false_iff in Heq. contradiction.
+Qed.
+
+(** Define one robot to get their location whenever they are gathered. *)
+Definition g1 : Names.G.
+Proof.
+exists 0. unfold N.nG. abstract (pose(Hle := Hyp_nG); omega).
+Defined.
+
+(** **  Description of similarities  **)
+
+(** Similarities can be described by [sim x = r A x + t] with:
+    - [0 < r] the ratio
+    - [t] the translation vector
+    - [A] an orthogonal matrix *)
+(* NB: To have less parameters, [r] is integrated into [A]. *)
+Open Scope R_scope.
+
+Theorem similarity_in_R2 : forall sim : Sim.t,
+  exists u v t, R2norm u = sim.(Sim.zoom) /\ R2norm v = sim.(Sim.zoom) /\ perpendicular u v /\
+    forall pt, sim pt = R2.add (R2.add (R2.mul (product u pt) u) (R2.mul (product v pt) v)) t.
+Proof.
+intros sim. exists (sim (1, 0) - sim (0, 0))%R2, (sim (0, 1) - sim (0, 0))%R2, (sim (0, 0)).
+repeat split.
+* rewrite <- R2norm_dist, sim.(Sim.dist_prop), <- Rmult_1_r. f_equal.
+  unfold R2.dist, R2def.dist, Rsqr. cbn.
+  ring_simplify ((1 - 0) * (1 - 0) + (0 - 0) * (0 - 0)). apply sqrt_1.
+* rewrite <- R2norm_dist, sim.(Sim.dist_prop), <- Rmult_1_r. f_equal.
+  unfold R2.dist, R2def.dist, Rsqr. cbn.
+  ring_simplify ((0 - 0) * (0 - 0) + (1 - 0) * (1 - 0)). apply sqrt_1.
+* assert (Hproduct : forall x y, 2 * product x y = (R2norm x)² + (R2norm y)² - (R2norm (x - y))²).
+  { intros x y. rewrite R2norm_sub. ring. }
+  unfold perpendicular. apply Rmult_eq_reg_l with 2; try lra.
+  rewrite Hproduct, Rmult_0_r.
+  repeat rewrite <- R2norm_dist. rewrite R2add_dist. repeat rewrite sim.(Sim.dist_prop).
+  repeat rewrite R_sqr.Rsqr_mult, square_dist_simpl. unfold Rsqr. cbn. ring.
+* intros [x y].
+  assert (H01 : ~R2.eq (0, 1) R2.origin).
+  { compute. intro Habs. inv Habs. now apply R1_neq_R0. }
+  rewrite (decompose_on H01 (x, y)) at 1.
+Admitted. (* similarity_in_R2 *)
+
+Corollary sim_add : forall (sim : Sim.t) x y, (sim (x + y) = sim x + sim y - sim R2.origin)%R2.
+Proof.
+intros sim x y. destruct (similarity_in_R2 sim) as [u [v [t [Hu [Hv [Huv Heq]]]]]].
+repeat rewrite Heq, ?product_origin_r, ?product_add_r, <- ?R2.add_morph, ?R2.mul_0.
+rewrite R2.add_origin, (R2.add_comm R2.origin t), R2.add_origin.
+repeat rewrite <- R2.add_assoc. rewrite R2.add_opp, R2.add_origin. f_equal.
+rewrite (R2.add_comm t). repeat rewrite R2.add_assoc. do 2 f_equal. apply R2.add_comm.
+Qed.
+
+Corollary sim_opp : forall (sim : Sim.t) x, (sim (- x) = 2 * sim R2.origin - sim x)%R2.
+Proof.
+intros sim x. apply (R2.add_reg_l (sim x)). apply (R2.add_reg_r (- sim R2.origin)).
+rewrite <- sim_add, R2.add_opp.
+setoid_rewrite R2.add_comm at 3. rewrite R2.add_assoc, R2.add_opp.
+setoid_rewrite R2.add_comm at 2. rewrite R2.add_origin.
+setoid_rewrite <- R2.mul_1 at 8. rewrite <- R2.minus_morph, R2.add_morph.
+ring_simplify (2 + -1). now rewrite R2.mul_1.
+Qed.
+
+Corollary sim_mul : forall (sim : Sim.t) k x, (sim (k * x) = k * sim x + (1 - k) * sim R2.origin)%R2.
+Proof.
+intros sim k x. destruct (similarity_in_R2 sim) as [u [v [t [Hu [Hv [Huv Heq]]]]]].
+repeat rewrite Heq, ?product_origin_r, ?product_mul_r, <- ?R2.add_morph, ?R2.mul_0.
+rewrite R2.add_origin, (R2.add_comm R2.origin t), R2.add_origin.
+repeat rewrite R2.mul_distr_add, ?R2.mul_morph. repeat rewrite <- R2.add_assoc. do 2 f_equal.
+rewrite R2.add_morph. ring_simplify (k + (1 - k)). now rewrite R2.mul_1.
+Qed.
+
+
+(** **  Definition of the robogram  **)
+
+Open Scope R_scope.
+Check Spect.multiplicity.
+(** The robogram solving the gathering problem in R². *)
+Definition ffgatherR2_pgm (s : Spect.t) : R2.t :=
+  wbarycenter (List.map (fun xn => (fst xn, INR (snd xn))) (Spect.M.elements s)).
+
+Instance ffgatherR2_pgm_compat : Proper (Spect.eq ==> R2.eq) ffgatherR2_pgm.
+Proof.
+intros ? ? Heq. unfold ffgatherR2_pgm. apply wbarycenter_compat.
+apply Spect.elements_compat in Heq.
+assert (Proper (Spect.eq_pair ==> R2.eq * eq) (fun xn : Spect.M.elt * nat => (fst xn, INR (snd xn)))).
+{ intros [] [] []. hnf in *; simpl in *. subst. split; reflexivity. }
+apply (Preliminary.PermutationA_map _ H Heq).
+Qed.
+
+Definition ffgatherR2 : robogram := {| pgm := ffgatherR2_pgm |}.
+
+Close Scope R_scope.
+
+
+(** **  Decreasing measure ensuring termination  **)
+
+(** ***  Global decreasing measure  **)
+
+
+Open Scope R_scope.
+
+(* Coercion Spect.Names.names : list Spect.Names.Internals.ident >-> list Spect.Names.ident. *)
+
+Definition max_dist_R2_pt_list (pt: R2.t) (l: list R2.t) : R :=
+  fold_right (fun pt1 max => Rmax (R2.dist pt pt1) max) 0 l.
+
+
+Lemma max_dist_R2_pt_list_le :
+  forall pt l pt1,
+    In pt1 l -> R2.dist pt pt1 <= max_dist_R2_pt_list pt l.
+Proof.
+  intros pt l pt1 Hin1.
+  induction l.
+  + elim Hin1.
+  + destruct Hin1.
+    - subst. unfold max_dist_R2_pt_list.
+      simpl.
+      apply Rmax_l.
+    - unfold max_dist_R2_pt_list. simpl.
+      unfold max_dist_R2_pt_list in IHl. apply IHl in H.
+      apply (Rle_trans _ _ _ H).
+      apply Rmax_r.
+Qed.
+
+Lemma max_dist_not_first :
+  forall pt pt1 l,
+    max_dist_R2_pt_list pt (pt1 :: l) <> R2.dist pt pt1 ->
+    l <> nil /\
+    max_dist_R2_pt_list pt (pt1 :: l) = max_dist_R2_pt_list pt l.
+Proof.
+  intros pt pt1 l Hnotfirst.
+  unfold max_dist_R2_pt_list in Hnotfirst.
+  simpl in Hnotfirst.
+  unfold Rmax at 1 in Hnotfirst.
+  unfold max_dist_R2_pt_list at 1. simpl.
+  unfold Rmax at 1.
+  destruct (Rle_dec (R2.dist pt pt1)
+                  (fold_right (fun (pt1 : R2.t) (max : R) => Rmax (R2.dist pt pt1) max) 0 l)).
+  split.
+  intro.
+  apply Hnotfirst.
+  rewrite H in *.
+  simpl in *.
+  assert (0 <= R2.dist pt pt1).
+  apply R2.dist_pos.
+  destruct H0.
+  assert (R2.dist pt pt1 < R2.dist pt pt1).
+  now apply Rle_lt_trans with (r2 := 0).
+  exfalso.
+  apply (Rlt_irrefl _ H1).
+  assumption.
+  reflexivity.
+  now elim Hnotfirst.
+Qed.
+
+Lemma max_dist_R2_pt_list_ex :
+  forall pt l,
+    l <> nil ->
+    exists pt1, In pt1 l /\ R2.dist pt pt1 = max_dist_R2_pt_list pt l.
+Proof.
+  intros pt l Hl.
+  induction l.
+  + now elim Hl.
+  + destruct (Req_dec (R2.dist pt a) (max_dist_R2_pt_list pt (a :: l))).
+    - exists a.
+      split.
+      now left.
+      assumption.
+    - assert (Hmax: max_dist_R2_pt_list pt (a::l) = max_dist_R2_pt_list pt l).
+      { apply max_dist_not_first.
+        intro. apply H. now rewrite H0. }
+      assert (Hlnotnil: l <> nil).
+      { generalize (max_dist_not_first pt a l).
+        intro.
+        apply H0.
+        intro. apply H. now rewrite H1. }
+      destruct (IHl Hlnotnil). destruct H0.
+      exists x.
+      split.
+      now right.
+      now rewrite Hmax.
+Qed.
+
+Lemma max_dist_R2_pt_list_0 : forall pt l, max_dist_R2_pt_list pt l = 0 <-> forall x, In x l -> x = pt.
+Proof.
+intros pt l. destruct l as [| pt' l].
+* cbn. tauto.
+* split; intro H.
+  + intros x Hin. assert (Hle := max_dist_R2_pt_list_le pt (pt' :: l) x Hin).
+    rewrite H in Hle. symmetry. rewrite <- R2.dist_defined. apply antisymmetry; trivial. apply R2.dist_pos.
+  + destruct (@max_dist_R2_pt_list_ex pt (pt' :: l) ltac:(discriminate)) as [? [Hin Heq]].
+    apply H in Hin. subst. rewrite <- Heq. apply R2_dist_defined_2.
+Qed.
+
+Definition max_dist_R2_list_list (l1: list R2.t) (l2: list R2.t): R :=
+  fold_right (fun pt0 max => Rmax max (max_dist_R2_pt_list pt0 l2)) 0 l1.
+
+Lemma max_dist_R2_list_list_le :
+  forall pt1 l1 pt2 l2,
+    In pt1 l1 -> In pt2 l2 -> R2.dist pt1 pt2 <= max_dist_R2_list_list l1 l2.
+Proof.
+  intros pt1 l1 pt2 l2 Hin1 Hin2.
+  induction l1.
+  + elim Hin1.
+  + destruct Hin1.
+    - subst. unfold max_dist_R2_list_list. simpl.
+      apply Rle_trans with (r2 := max_dist_R2_pt_list pt1 l2).
+      now apply max_dist_R2_pt_list_le.
+      now apply Rmax_r.
+    - unfold max_dist_R2_list_list. simpl.
+      apply IHl1 in H.
+      apply (Rle_trans _ _ _ H).
+      now apply Rmax_l.
+Qed.
+
+Lemma max_dist_R2_list_list_ex :
+  forall l1 l2,
+    l1 <> nil ->
+    l2 <> nil ->
+    exists pt1 pt2, In pt1 l1 /\ In pt2 l2 /\ R2.dist pt1 pt2 = max_dist_R2_list_list l1 l2.
+Proof.
+  intros l1 l2 Hl1notnil Hl2notnil.
+  induction l1.
+  + now elim Hl1notnil.
+  + unfold max_dist_R2_list_list.
+    simpl.
+    unfold Rmax at 1.
+    destruct (Rle_dec (fold_right (fun (pt0 : R2.t) (max : R) => Rmax max (max_dist_R2_pt_list pt0 l2)) 0 l1)
+         (max_dist_R2_pt_list a l2)).
+    - exists a.
+      destruct (max_dist_R2_pt_list_ex a Hl2notnil) as [? [? ?]].
+      exists x. split.
+      now left.
+      now split.
+    - clear Hl1notnil.
+      assert (Hl1notnil: l1 <> nil).
+      { intro. apply n. subst. simpl.
+        induction l2.
+        unfold max_dist_R2_pt_list. simpl. apply Rle_refl.
+        simpl. apply Rle_trans with (r2 := R2.dist a a0).
+        apply R2.dist_pos.
+        apply Rmax_l. }
+      destruct (IHl1 Hl1notnil) as [? [? [? [? ?]]]].
+      exists x, x0.
+      split.
+      now right.
+      now split.
+Qed.
+
+Lemma max_dist_R2_list_list_cons_le : forall pt l,
+  max_dist_R2_list_list l l <= max_dist_R2_list_list (pt :: l) (pt :: l).
+Proof.
+intros pt [| pt' l].
+- cbn. rewrite R2_dist_defined_2. now repeat rewrite Rmax_left.
+- destruct (@max_dist_R2_list_list_ex (pt' :: l) (pt' :: l))
+    as [pt1 [pt2 [Hpt1 [Hpt2 Heq]]]]; try discriminate; [].
+  rewrite <- Heq. apply max_dist_R2_list_list_le; now right.
+Qed.
+
+Definition max_dist_spect (spect: Spect.t) : R :=
+  max_dist_R2_list_list (Spect.support spect) (Spect.M.support spect).
+
+Lemma max_dist_spect_le :
+  forall (spect: Spect.t) pt0 pt1,
+    InA R2.eq pt0 (Spect.support spect) ->
+    InA R2.eq pt1 (Spect.support spect) ->
+    R2.dist pt0 pt1 <= max_dist_spect spect.
+Proof. setoid_rewrite InA_Leibniz. intros. now apply max_dist_R2_list_list_le. Qed.
+
+Lemma max_dist_spect_ex :
+  forall (spect: Spect.t),
+    Spect.M.support spect <> nil ->
+    exists pt0 pt1, 
+      In pt0 (Spect.M.support spect)
+      /\ In pt1 (Spect.M.support spect)
+      /\ R2.dist pt0 pt1 = max_dist_spect spect.
+Proof. intros. now apply max_dist_R2_list_list_ex. Qed.
+
+
+(** **  Main result for termination: the measure decreases after a step where a robot moves  *)
+
+Definition measure (conf: Config.t) : R :=
+  max_dist_spect (!! conf).
+
+Lemma measure_nonneg : forall config, 0 <= measure config.
+Proof.
+intros config. unfold measure.
+destruct (Spect.M.support (!! config)) as [| pt l] eqn:Heq.
++ elim (support_non_nil _ Heq).
++ rewrite <- (R2_dist_defined_2 pt). apply max_dist_spect_le; rewrite Heq; now left.
+Qed.
+
+Lemma gathered_support : forall config pt,
+  gathered_at pt config <-> PermutationA R2.eq (Spect.M.support (!! config)) (pt :: nil).
+Proof.
+intros config pt. split; intro H.
+* apply NoDupA_equivlistA_PermutationA; autoclass.
+  + apply Spect.M.support_NoDupA.
+  + repeat constructor. intro Hin. inv Hin.
+  + intro pt'. split; intro Hin.
+    - rewrite Spect.M.support_In, (Spect.from_config_In config pt') in Hin.
+      destruct Hin as [id Hid]. revert Hid. apply (no_byz id). clear id; intros g Hid.
+      specialize (H g). rewrite H in Hid. rewrite Hid. now left.
+    - inv Hin; try inv H1; [].
+      rewrite Spect.M.support_In, (Spect.from_config_In config pt).
+      exists (Good g1). apply H.
+* intro id.
+  assert (Hin : InA eq (Config.loc (config (Good id))) (Spect.M.support (!! config))).
+  { rewrite Spect.M.support_In. apply (Spect.from_config_In config). eexists; reflexivity. }
+  rewrite H in Hin. now inv Hin.
+Qed.
+
+Lemma gathered_measure : forall config, measure config = 0 <-> exists pt, gathered_at pt config.
+Proof.
+intros config. split; intro H.
+* unfold measure, max_dist_spect in *.
+  assert (Hnil := support_non_nil config).
+  assert (Hdup := Spect.M.support_NoDupA (!! config)).
+  setoid_rewrite gathered_support.
+  induction (Spect.M.support (!! config)) as [| pt l]; try tauto; [].
+  exists pt. destruct l; try reflexivity.
+  inv Hdup. destruct IHl; discriminate || auto.
+  + apply antisymmetry.
+    - rewrite <- H. apply max_dist_R2_list_list_cons_le.
+    - rewrite <- (R2_dist_defined_2 e). apply max_dist_R2_list_list_le; now left.
+  + assert (l = nil).
+    { rewrite <- length_zero_iff_nil.
+      cut (length (e :: l) = length (x :: nil)); try (simpl; omega).
+      f_equiv; eauto. }
+    subst. rewrite PermutationA_1 in H0; autoclass; []. subst.
+    elim H2. left.
+    cbn in H. do 2 rewrite R2_dist_defined_2 in H.
+    rewrite (Rmax_left 0 0) in H; try reflexivity; [].
+    rewrite R2.dist_sym in H.
+    match type of H with Rmax ?x ?x = 0 => rewrite (Rmax_left x) in H; try reflexivity end.
+    rewrite (Rmax_right 0), Rmax_left in H.
+    - now rewrite R2.dist_defined in H.
+    - apply R2.dist_pos.
+    - rewrite Rmax_left; apply R2.dist_pos.
+* destruct H as [pt Hgather]. unfold measure.
+  destruct (max_dist_spect_ex (support_non_nil config)) as [pt1 [pt2 [Hpt1 [Hpt2 Heq]]]].
+  rewrite <- Heq, R2.dist_defined. rewrite gathered_support in Hgather. rewrite <- InA_Leibniz, Hgather in *.
+  now inv Hpt1; inv Hpt2.
+Qed.
+
+Lemma fold_mult_plus_distr : forall (f : R2.t -> R) coeff E init,
+  fold_left (fun acc pt => acc + snd pt * coeff * (f (fst pt))) E (coeff * init) =
+  coeff * (fold_left (fun acc pt => acc + snd pt * (f (fst pt))) E init).
+Proof.
+  intros f coeff E.
+  induction E; intro init.
+  + now simpl.
+  + simpl. rewrite <- IHE. f_equal. ring.
+Qed.
+
+Lemma wbarycenter_sim : forall (sim : Sim.t) m,
+    m <> nil ->
+    R2.eq (wbarycenter (map (fun xn => (sim (fst xn), snd xn)) m)) (sim (wbarycenter m)).
+Proof.
+  intros sim m Hm. eapply wbarycenter_n_unique.
+  + apply wbarycenter_n_spec.
+  + intro p.
+    unfold weighted_sqr_dist_sum.
+    change p with (Sim.id p).
+    rewrite <- (Sim.compose_inverse_r sim) with (x := p) by apply R2.eq_equiv.
+    change ((Sim.compose sim (sim ⁻¹)) p) with (sim ((sim ⁻¹) p)).
+
+    assert (Hfold_dist_prop: forall pt init,
+              fold_left (fun acc pt' => acc + snd pt'* (R2.dist (sim pt) (fst pt'))²)
+                        (map (fun xn => (Bijection.section (Common.Sim.sim_f sim) (fst xn), snd xn)) m) init
+            = fold_left (fun acc pt' => acc + snd pt' * (sim.(Sim.zoom))² * (R2.dist pt (fst pt'))²) m init).
+    { intro pt. induction m as [| p1 m]; intro init.
+      + now elim Hm.
+      + clear Hm. destruct m as [| p2 m].
+        * simpl.
+          rewrite sim.(Sim.dist_prop), R_sqr.Rsqr_mult. ring.
+        * remember (p2 :: m) as mm.
+          simpl.
+          rewrite sim.(Sim.dist_prop), R_sqr.Rsqr_mult.
+          rewrite IHm.
+          - f_equal. ring.
+          - subst. discriminate.
+    }
+    do 2 rewrite Hfold_dist_prop.
+    rewrite <- Rmult_0_r with (r := (Sim.zoom sim)²).
+    rewrite (fold_mult_plus_distr (fun x => (R2.dist (wbarycenter m) x)²)),
+            (fold_mult_plus_distr (fun x => (R2.dist (Bijection.section (Common.Sim.sim_f (sim ⁻¹)) p) x)²)).
+    apply Rmult_le_compat_l.
+    - apply Rle_0_sqr.
+    - generalize (wbarycenter_n_spec m).
+      intro Hbary_spec.
+      unfold is_wbarycenter_n, weighted_sqr_dist_sum in Hbary_spec.
+      now apply Hbary_spec.
+Qed.
+
+Lemma dist_prop_retraction:
+  forall (sim: Sim.t) (x y : R2.t),
+    R2.dist ((Sim.sim_f (sim ⁻¹)) x) ((Sim.sim_f (sim ⁻¹)) y) =
+    /(Sim.zoom sim) * R2.dist x y.
+Proof. intros sim x y. rewrite Sim.dist_prop. now simpl. Qed.
+
+Theorem round_simplify : forall da config delta,
+    Config.eq (round delta ffgatherR2 da config)
+              (fun id => match da.(step) id with
+                         | None => config id
+                         | Some (f, r) =>
+                           let bary := wbarycenter (List.map (fun xn => (fst xn, INR (snd xn)))
+                                                             (Spect.elements (!! config))) in
+                           let move := (r * (bary - (config id)))%R2 in
+                             mk_info (if Rle_bool delta (R2norm move)
+                                      then ((config id) + move)%R2
+                                      else bary)
+                         end).
+Proof.
+intros da config delta. apply no_byz_eq. intro g. hnf. unfold round.
+assert (supp_nonempty:=support_non_nil config).
+destruct (step da (Good g)) as [[f r] |] eqn:Hstep; trivial.
+remember (Config.loc (config (Good g))) as pt. remember (f pt) as sim.
+assert (Hsim : Proper (R2.eq ==> R2.eq) sim). { intros ? ? Heq. now rewrite Heq. }
+simpl pgm. unfold ffgatherR2_pgm.
+assert (Hperm : PermutationA (R2.eq * eq)%signature
+                             (map (fun xn => (sim (fst xn), snd xn)) (Spect.M.elements (!! config)))
+                             (Spect.M.elements (!! (Config.map (Config.app sim) config)))).
+{ now rewrite <- map_sim_elements, Spect.from_config_map. }
+change Common.Sim.sim_f with Sim.sim_f.
+remember (List.map (fun xn => (fst xn, INR (snd xn))) (Spect.M.elements (!! config))) as E.
+remember (List.map (fun xn => (fst xn, INR (snd xn)))
+                   (Spect.M.elements (!! (Config.map (Config.app sim) config)))) as E'.
+rewrite R2norm_mul, <- R2norm_dist.
+assert (Hsimbary : (sim ⁻¹) (wbarycenter E') = wbarycenter E).
+{ rewrite HeqE' in *.
+  rewrite <- wbarycenter_sim.
+  + apply wbarycenter_compat.
+    rewrite map_map. simpl.
+    rewrite <- (map_map (fun xn => (Bijection.retraction (Common.Sim.sim_f sim) (fst xn), snd xn))
+                        (fun xn => (fst xn, INR (snd xn)))).
+    rewrite HeqE. apply (PermutationA_map (eqA := R2.eq * eq)%signature);
+    autoclass; try (now intros [] [] []; hnf in *; simpl in * |-; split; subst); [].
+    rewrite <- Spect.map_injective_elements; autoclass.
+    - rewrite Spect.from_config_map, Config.map_merge; autoclass; [].
+      do 2 f_equiv.
+      rewrite <- (Config.map_id config) at 2. f_equiv.
+      intros x y Hxy.
+      rewrite <- (Config.app_id y); try reflexivity; [].
+      change (Config.app id y) with (Config.app Sim.id y).
+      rewrite <- (Sim.compose_inverse_l sim).
+      symmetry. simpl. apply Config.app_compose; autoclass; now symmetry.
+    - change (Bijection.retraction sim) with (Bijection.section (sim ⁻¹)).
+      apply Sim.injective.
+  + rewrite <- length_zero_iff_nil, map_length, <- Spect.from_config_map; autoclass.
+    rewrite Spect.map_injective_elements; autoclass; try apply Sim.injective.
+    rewrite map_length, length_zero_iff_nil, Spect.elements_nil. apply spect_non_nil. }
+assert (Htest : Rle_bool delta (R2.dist ((sim ⁻¹) (r * wbarycenter E')%R2) pt)
+                = Rle_bool delta (Rabs r * R2.dist (wbarycenter E) pt)).
+{ f_equal.
+  assert (Heq_pt : pt = (sim ⁻¹) (sim pt)).
+  { simpl. rewrite Bijection.retraction_section; autoclass. }
+  assert (Hsim_pt : R2.eq (sim pt) (r * (sim pt))).
+  { generalize (Sim.center_prop sim).
+    intro Hzero.
+    apply step_center with (c := pt) in Hstep.
+    simpl in Hstep. rewrite <- Heqsim in Hstep.
+    now rewrite <- Hstep, Hzero, R2.mul_origin. }
+  rewrite Heq_pt at 1.
+  rewrite dist_prop_retraction, Hsim_pt, R2mul_dist, <- Rmult_assoc.
+  pattern (/ Sim.zoom sim * Rabs r).
+  rewrite Rmult_comm, Rmult_assoc. f_equal.
+  rewrite <- dist_prop_retraction, <- Heq_pt. f_equal. assumption. }
+rewrite Htest.
+destruct (Rle_bool delta (Rabs r * R2.dist (wbarycenter E) pt)); trivial; [].
+apply Bijection.Inversion.
+simpl Bijection.retraction. change Common.Sim.sim_f with Sim.sim_f.
+rewrite sim_add, sim_mul, sim_add, sim_opp.
+do 2 rewrite R2.mul_distr_add.
+assert (Hsim_pt_0 : R2.eq (sim pt) R2.origin).
+{ apply (step_center da (Good g) pt) in Hstep.
+  rewrite <- sim.(Sim.center_prop), <- Hstep. cbn. now subst sim. }
+rewrite Hsim_pt_0.
+rewrite (R2.add_comm R2.origin), R2.add_origin.
+setoid_rewrite <- R2.add_origin at 25. repeat rewrite <- R2.add_assoc. f_equiv.
++ f_equiv. rewrite Bijection.Inversion. apply Hsimbary.
++ rewrite R2.opp_origin, R2.add_origin.
+  setoid_rewrite <- R2.mul_1 at 9 15. repeat rewrite <- ?R2.minus_morph, ?R2.mul_morph, ?R2.add_morph.
+  ring_simplify (r * 2 + (r * -1 + (1 - r + -1))). apply R2.mul_0.
+Qed.
+
+
+(* FIXME: cleanup! *)
+Theorem round_lt_config : forall d conf delta,
+    delta > 0 ->
+    FullySynchronous d ->
+    delta <= measure conf ->
+    measure (round delta ffgatherR2 (Stream.hd d) conf) <= measure conf - delta.
+Proof.
+  assert (Proper (Spect.eq_pair ==> R2.eq * eq) (fun xn => (fst xn, INR (snd xn)))).
+  { clear. intros [] [] []. hnf in *; simpl in *. now subst. }
+  intros d conf delta Hdelta HFSync Hnotdone.
+  destruct (Spect.elements (!! conf)) as [| [pt n] [| [pt' n'] ?]] eqn:Hmax.
+  - (* No robots *)
+    exfalso. apply (support_non_nil conf), (@PermutationA_nil _ R2.eq _).
+    now rewrite Spect.support_map_elements, Hmax.
+  - (* Done *)
+    assert (Habs : measure conf = 0).
+    { rewrite gathered_measure. exists pt. rewrite gathered_support.
+      now rewrite Spect.support_map_elements, Hmax. }
+    rewrite Habs in *. elim (Rlt_irrefl delta). now apply Rle_lt_trans with 0.
+  - (* Now to some real work *)
+    remember (Stream.hd d) as da.
+    remember (Spect.elements (!! conf)) as elems.
+    remember (map (fun xn => (fst xn, INR (snd xn))) elems) as relems.
+    set (C := wbarycenter relems).
+    remember (Spect.elements (!! (round delta ffgatherR2 da conf))) as nxt_elems.
+    assert (Hantec: forall KP, InA Spect.eq_elt KP nxt_elems ->
+              exists Pid k, InA Spect.eq_elt (Config.loc (conf Pid), k) elems
+                         /\ R2.eq (round delta ffgatherR2 da conf Pid) (fst KP)).
+    { intros [KP k'] HinKP.
+      rewrite Heqnxt_elems in HinKP.
+      rewrite Spect.elements_In in HinKP.
+      generalize (Spect.from_config_In (round delta ffgatherR2 da conf)).
+      intro Hok. rewrite Hok in HinKP. clear Hok.
+      destruct HinKP as (Pid, HPid).
+      exists Pid, k'.
+      split; [|now rewrite HPid].
+      rewrite Heqelems, Spect.elements_In, Spect.from_config_In.
+      now exists Pid.
+    }
+
+    assert (Hrobot_move_less_than_delta:
+              forall Pid k,
+                InA Spect.eq_elt (Config.loc (conf Pid), k) elems ->
+                delta > R2.dist (conf Pid) C ->
+                R2.eq (round delta ffgatherR2 da conf Pid) C).
+    { intros Pid k HinP HdeltaP.
+      rewrite (round_simplify _ _ _ Pid).
+      destruct (step da Pid) eqn:HeqPact.
+      + simpl.
+        destruct (Spect.M.elements (!! conf)) as [| q [| q' ?]].
+        - subst elems. inversion Hmax.
+        - subst elems. inversion Hmax.
+        - rewrite <- Heqelems, <- Heqrelems.
+          destruct p.
+          unfold Rle_bool.
+          destruct (Rle_dec delta (R2norm (r * (wbarycenter relems - conf Pid)))) as [ Hdmove | Hdmove ].
+          * assert (Hr: 0 <= snd (t, r) <= 1).
+            { apply (step_flexibility da Pid). now symmetry. } simpl in Hr.
+            destruct Hr as [Hr0 Hr1].
+            destruct Hr1.
+            ++ exfalso.
+               rewrite R2norm_mul in Hdmove.
+               rewrite <- R2norm_dist in Hdmove.
+               rewrite R2.dist_sym in Hdmove.
+               apply Rlt_irrefl with (r := delta).
+               apply (Rle_lt_trans _ _ _ Hdmove).
+               apply Rgt_lt in HdeltaP.
+               apply Rlt_trans with (r2 := R2.dist (conf Pid) C);
+                 [ | assumption].
+               rewrite <- Rmult_1_l.
+               apply Rmult_lt_compat_r.
+               -- apply Rlt_le_trans with (r2 := delta).
+                  ** now apply Rgt_lt.
+                  ** apply (Rle_trans _ _ _ Hdmove).
+                     rewrite <- Rmult_1_l.
+                     apply Rmult_le_compat_r.
+                     +++ apply R2.dist_pos.
+                     +++ apply Rabs_le.
+                         split.
+                     --- apply Rle_trans with (r2 := -0).
+                         apply Ropp_ge_le_contravar.
+                         apply Rle_ge.
+                         apply Rle_0_1.
+                         now rewrite Ropp_0.
+                     --- now left.
+               -- apply Rabs_def1. assumption. apply Rlt_le_trans with (r2 := 0).
+                  apply Rlt_le_trans with (r2 := -0).
+                  apply Ropp_gt_lt_contravar.
+                  apply Rlt_gt.
+                  apply Rlt_0_1.
+                  now rewrite Ropp_0.  assumption.
+            ++ subst r. rewrite R2.mul_1.
+               rewrite R2.add_assoc.
+               pattern (conf Pid + wbarycenter relems)%R2.
+               rewrite R2.add_comm.
+               rewrite <- R2.add_assoc.
+               rewrite R2.add_opp.
+               rewrite R2.add_origin.
+               now subst C.
+          * now subst C.
+      + unfold FullySynchronous in HFSync.
+        unfold FullySynchronousInstant in HFSync.
+        destruct d.
+        simpl in Heqda.
+        destruct HFSync.
+        destruct (H0 Pid).
+        simpl.
+        subst d.
+        now symmetry.
+    }
+
+    assert (Hrobot_move:
+              forall Pid k,
+                InA Spect.eq_elt (Config.loc (conf Pid), k) elems ->
+                delta <= R2.dist (conf Pid) C ->
+                exists k, R2.eq (round delta ffgatherR2 da conf Pid)
+                                (conf Pid + k * (C - (conf Pid)))%R2
+                       /\ 0 <= k <= 1
+                       /\ delta <= R2norm (k * (C - (conf Pid)))).
+    { intros Pid HinP HdeltaP.
+      setoid_rewrite (round_simplify _ _ _ Pid).
+      remember (step da Pid) as Pact.
+      destruct Pact.
+      + destruct (Spect.M.elements (!! conf)) as [| q [| q' ?]].
+        - subst elems. inversion Hmax.
+        - subst elems. inversion Hmax.
+        - rewrite <- Heqelems, <- Heqrelems.
+          destruct p.
+          unfold Rle_bool.
+          destruct (Rle_dec delta (R2norm (r * (wbarycenter relems - conf Pid)))) as [ Hdmove | Hdmove ].
+          * assert (Hr: 0 <= snd (t, r) <= 1).
+            { apply (step_flexibility da Pid). now symmetry. } simpl in Hr.
+            exists r.
+            repeat split; tauto.
+          * exists 1.
+            repeat split.
+            ++ rewrite R2.mul_1.
+               rewrite R2.add_comm.
+               rewrite <- R2.add_assoc.
+               pattern (- conf Pid + conf Pid)%R2.
+               now rewrite R2.add_comm, R2.add_opp, R2.add_origin.
+            ++ apply Rle_0_1.
+            ++ apply Rle_refl.
+            ++ now rewrite R2.mul_1, <- R2norm_dist, R2.dist_sym.
+      + unfold FullySynchronous in HFSync.
+        unfold FullySynchronousInstant in HFSync.
+        destruct d.
+        simpl in Heqda.
+        destruct HFSync.
+        destruct (H0 Pid).
+        simpl.
+        subst d.
+        now symmetry.
+    }
+
+    assert (MainArgument: forall KP KQ, InA Spect.eq_elt KP nxt_elems -> InA Spect.eq_elt KQ nxt_elems ->
+            R2.dist (fst KP) (fst KQ) <= max_dist_spect (!! conf) - delta).
+    { intros KP KQ HinKP HinKQ.
+      apply Hantec in HinKP.
+      apply Hantec in HinKQ.
+      destruct HinKP as [Pid [kP [HinP HroundP]]],
+               HinKQ as [Qid [kQ [HinQ HroundQ]]].
+
+      destruct (Rle_dec delta (R2.dist (conf Pid) C)), (Rle_dec delta (R2.dist (conf Qid) C)).
+      + generalize HinP.
+        apply Hrobot_move in HinP; [|assumption].
+        intro HinPP.
+        generalize HinQ.
+        apply Hrobot_move in HinQ; [|assumption].
+        intro HinQQ.
+        destruct HinP as [kp [kp_def [Hkple1 Hkplow]]].
+        destruct HinQ as [kq [kq_def [Hkqle1 Hkqlow]]].
+        rewrite kp_def in HroundP.
+        rewrite kq_def in HroundQ.
+
+        assert (HPnotC: ~ R2.eq (conf Pid) C).
+        { intro.
+          apply (Rlt_irrefl 0).
+          apply Rlt_le_trans with (r2 := delta).
+          assumption.
+          apply R2.dist_defined in H0.
+          rewrite H0 in r.
+          assumption. }
+        assert (HQnotC: ~ R2.eq (conf Qid) C).
+        { intro.
+          apply (Rlt_irrefl 0).
+          apply Rlt_le_trans with (r2 := delta).
+          assumption.
+          apply R2.dist_defined in H0.
+          rewrite H0 in r0.
+          assumption. }
+
+        destruct (Rle_dec kp kq).
+        - apply Rle_trans with (r2 := (1 - kp) * (max_dist_spect (!! conf))).
+          * rewrite <- HroundP in *. rewrite <- HroundQ in *. clear HroundP HroundQ KP KQ.
+            apply distance_after_move; try assumption.
+            ** subst C. change (conf Pid) with (fst (conf Pid, INR kP)).
+               eapply (@wbarycenter_dist_decrease relems (max_dist_spect (!! conf)))
+                 with (p := (Config.loc (conf Pid), INR kP)).
+               ++ subst relems elems. intro Habs. apply map_eq_nil in Habs.
+                  rewrite Habs, InA_nil in *. tauto.
+               ++ subst relems elems. intro.
+                  rewrite (InA_map_iff (eqA := Spect.eq_pair)); autoclass; [].
+                  intros [[pta na] [Heq Hin]]. rewrite Spect.elements_spec in Hin.
+                  destruct p, Heq. simpl in *. subst. now apply lt_0_INR.
+               ++ intros p1 p2 Hin1 Hin2. subst relems elems.
+                  rewrite InA_map_iff in Hin1, Hin2; autoclass; [].
+                  apply max_dist_spect_le.
+                  -- rewrite Spect.support_map_elements, InA_map_iff; autoclass; [].
+                     destruct Hin1 as [p1' [Heq1 Hin1]].
+                     exists p1'. split; trivial; []. destruct p1', Heq1 as [Heq1 _].
+                     now hnf in *; simpl in *.
+                  -- rewrite Spect.support_map_elements, InA_map_iff; autoclass; [].
+                     destruct Hin2 as [p2' [Heq2 Hin2]].
+                     exists p2'. split; trivial; []. destruct p2', Heq2 as [Heq2 _].
+                     now hnf in *; simpl in *.
+               ++ subst relems. rewrite (@InA_map_iff _ _ Spect.eq_elt); autoclass.
+                  -- now exists (Config.loc (conf Pid), kP).
+                  -- clear. intros [] [] ?. now hnf in *; simpl in *.
+            ** 
+++
+            now subst elems.
+            now subst elems.
+            destruct (Rlt_dec 0 kp); try assumption.
+            exfalso.
+            apply n.
+            destruct Hkple1 as [[Hkplt0 | Hkpeq0] _].
+            assumption.
+            subst kp.
+            apply Rlt_le_trans with (r2 := delta).
+            assumption.
+            rewrite R2.mul_0 in Hkplow.
+            rewrite R2norm_origin in Hkplow.
+            assumption.
+            now destruct Hkqle1.
+          * rewrite Rmult_comm.
+            rewrite Rmult_minus_distr_l.
+            rewrite Rmult_1_r.
+            apply Rplus_le_compat_l.
+            apply Ropp_ge_le_contravar.
+            apply Rle_ge.
+            apply (Rle_trans _ _ _ Hkplow).
+            rewrite R2norm_mul.
+            rewrite Rabs_pos_eq.
+            rewrite Rmult_comm.
+            apply Rmult_le_compat_r.
+            now destruct Hkple1.
+            rewrite <- R2norm_dist.
+            rewrite R2.dist_sym.
+            apply barycenter_dist_decrease with (E := elems).
+            subst elems.
+            rewrite Hmax; intro; discriminate.
+            intros. apply max_dist_spect_le.
+            now subst elems.
+            now subst elems.
+            now subst C.
+            assumption.
+            now destruct Hkple1.
+        - apply Rle_trans with (r2 := (1 - kq) * (max_dist_spect (!! conf))).
+          * rewrite <- HroundP in *. rewrite <- HroundQ in *. clear HroundP HroundQ KP KQ.
+            rewrite R2.dist_sym.
+            apply distance_after_move; try assumption.
+            apply barycenter_dist_decrease with (E := elems).
+            subst elems.
+            rewrite Hmax; intro; discriminate.
+            clear n.
+            intros. apply max_dist_spect_le.
+            now subst elems.
+            now subst elems.
+            now subst C.
+            assumption.
+            apply max_dist_spect_le.
+            now subst elems.
+            now subst elems.
+            destruct (Rlt_dec 0 kq); try assumption.
+            exfalso.
+            apply n0.
+            destruct Hkqle1 as [[Hkqlt0 | Hkqeq0] _].
+            assumption.
+            subst kq.
+            apply Rlt_le_trans with (r2 := delta).
+            assumption.
+            rewrite R2.mul_0 in Hkqlow.
+            rewrite R2norm_origin in Hkqlow.
+            assumption.
+            left. now apply Rnot_le_lt.
+            now destruct Hkple1.
+          * rewrite Rmult_comm.
+            rewrite Rmult_minus_distr_l.
+            rewrite Rmult_1_r.
+            apply Rplus_le_compat_l.
+            apply Ropp_ge_le_contravar.
+            apply Rle_ge.
+            apply (Rle_trans _ _ _ Hkqlow).
+            rewrite R2norm_mul.
+            rewrite Rabs_pos_eq.
+            rewrite Rmult_comm.
+            apply Rmult_le_compat_r.
+            now destruct Hkqle1.
+            rewrite <- R2norm_dist.
+            rewrite R2.dist_sym.
+            apply barycenter_dist_decrease with (E := elems).
+            subst elems.
+            rewrite Hmax; intro; discriminate.
+            intros. apply max_dist_spect_le.
+            now subst elems.
+            now subst elems.
+            now subst C.
+            assumption.
+            now destruct Hkqle1.
+
+      + generalize HinP.
+        apply Hrobot_move in HinP; [|assumption].
+        intro HinPP.
+        generalize HinQ.
+        apply Hrobot_move_less_than_delta in HinQ.
+        intro HinQQ.
+        destruct HinP as [kp [kp_def [Hkple1 Hkplow]]].
+        rewrite kp_def in HroundP.
+        rewrite HinQ in HroundQ.
+
+        rewrite <- HroundP in *. rewrite <- HroundQ in *. clear HroundP HroundQ KP KQ.
+        apply Rle_trans with (r2 := R2.dist (conf Pid) C - delta).
+        rewrite R2norm_dist.
+        assert (conf Pid + kp * (C - conf Pid) - C = (1 + - kp) * (conf Pid - C))%R2.
+        { symmetry. rewrite <- R2.add_morph.
+          rewrite R2.mul_1.
+          replace (conf Pid - C)%R2 with (- (C - conf Pid))%R2 at 2.
+          rewrite R2.mul_opp.
+          rewrite R2.minus_morph.
+          rewrite R2.opp_opp.
+          rewrite <- R2.add_assoc.
+          rewrite R2.add_comm with (u := (-C)%R2).
+          now rewrite R2.add_assoc.
+          rewrite R2.opp_distr_add.
+          rewrite R2.opp_opp.
+          now rewrite R2.add_comm.
+        }
+        rewrite H.
+        rewrite R2norm_mul.
+        rewrite R2norm_dist.
+        rewrite Rabs_pos_eq.
+        rewrite Rmult_plus_distr_r.
+        rewrite Rmult_1_l.
+        apply Rplus_le_compat_l.
+        rewrite <- Ropp_mult_distr_l.
+        apply Ropp_ge_le_contravar.
+        apply Rle_ge.
+        rewrite <- R2norm_dist.
+        rewrite R2.dist_sym.
+        rewrite R2norm_dist.
+        rewrite <- Rabs_pos_eq with (x := kp).
+        now rewrite <- R2norm_mul.
+        now destruct Hkple1.
+        apply Rplus_le_reg_r with (r := kp).
+        rewrite Rplus_0_l.
+        rewrite Rplus_assoc.
+        rewrite Rplus_opp_l.
+        rewrite Rplus_0_r.
+        now destruct Hkple1.
+        apply Rplus_le_compat_r.
+        apply barycenter_dist_decrease with (E := elems).
+        subst elems.
+        rewrite Hmax; intro; discriminate.
+        intros. apply max_dist_spect_le.
+        now subst elems.
+        now subst elems.
+        now subst C.
+        assumption.
+        now apply Rnot_le_gt.
+
+      + generalize HinQ.
+        apply Hrobot_move in HinQ; [|assumption].
+        intro HinQQ.
+        generalize HinP.
+        apply Hrobot_move_less_than_delta in HinP.
+        intro HinPP.
+        destruct HinQ as [kq [kq_def [Hkqle1 Hkqlow]]].
+        rewrite kq_def in HroundQ.
+        rewrite HinP in HroundP.
+
+        rewrite <- HroundP in *. rewrite <- HroundQ in *. clear HroundP HroundQ KP KQ.
+        apply Rle_trans with (r2 := R2.dist (conf Qid) C - delta).
+        rewrite R2.dist_sym.
+        rewrite R2norm_dist.
+        assert (conf Qid + kq * (C - conf Qid) - C = (1 + - kq) * (conf Qid - C))%R2.
+        { symmetry. rewrite <- R2.add_morph.
+          rewrite R2.mul_1.
+          replace (conf Qid - C)%R2 with (- (C - conf Qid))%R2 at 2.
+          rewrite R2.mul_opp.
+          rewrite R2.minus_morph.
+          rewrite R2.opp_opp.
+          rewrite <- R2.add_assoc.
+          rewrite R2.add_comm with (u := (-C)%R2).
+          now rewrite R2.add_assoc.
+          rewrite R2.opp_distr_add.
+          rewrite R2.opp_opp.
+          now rewrite R2.add_comm.
+        }
+        rewrite H.
+        rewrite R2norm_mul.
+        rewrite R2norm_dist.
+        rewrite Rabs_pos_eq.
+        rewrite Rmult_plus_distr_r.
+        rewrite Rmult_1_l.
+        apply Rplus_le_compat_l.
+        rewrite <- Ropp_mult_distr_l.
+        apply Ropp_ge_le_contravar.
+        apply Rle_ge.
+        rewrite <- R2norm_dist.
+        rewrite R2.dist_sym.
+        rewrite R2norm_dist.
+        rewrite <- Rabs_pos_eq with (x := kq).
+        now rewrite <- R2norm_mul.
+        now destruct Hkqle1.
+        apply Rplus_le_reg_r with (r := kq).
+        rewrite Rplus_0_l.
+        rewrite Rplus_assoc.
+        rewrite Rplus_opp_l.
+        rewrite Rplus_0_r.
+        now destruct Hkqle1.
+        apply Rplus_le_compat_r.
+        apply barycenter_dist_decrease with (E := elems).
+        subst elems.
+        rewrite Hmax; intro; discriminate.
+        intros. apply max_dist_spect_le.
+        now subst elems.
+        now subst elems.
+        now subst C.
+        assumption.
+        now apply Rnot_le_gt.
+
+      + apply Hrobot_move_less_than_delta in HinP.
+        apply Hrobot_move_less_than_delta in HinQ.
+        rewrite <- HroundP in *. rewrite <- HroundQ in *. clear HroundP HroundQ KP KQ.
+        rewrite HinP, HinQ.
+        assert (R2.dist C C = 0).
+        { rewrite R2.dist_defined. apply R2.eq_equiv. }
+        rewrite H.
+        apply Rplus_le_reg_r with (r := delta).
+        rewrite Rplus_0_l.
+        assert (max_dist_spect (!! conf) - delta + delta = max_dist_spect (!! conf)) by ring.
+        rewrite H0.
+        apply Hnotdone.
+        now apply Rnot_le_gt.
+        now apply Rnot_le_gt.
+    }
+
+    unfold measure.
+    generalize (max_dist_spect_ex (!!(round delta ffgatherR2 da conf))).
+    intros Hmax_dist_ex.
+    assert (Hspect_non_nil: nxt_elems <> nil).
+    { rewrite Heqnxt_elems.
+      apply support_non_nil. }
+    rewrite <- Heqnxt_elems in Hmax_dist_ex.
+    destruct (Hmax_dist_ex Hspect_non_nil) as [pt0 [pt1 [Hin0 [Hin1 Hdist]]]].
+    rewrite <- Hdist.
+    now auto.
+Qed.
+
+(* FIXME: cleanup! *)
+Theorem round_last_step : forall d conf delta,
+    delta > 0 ->
+    FullySynchronous d ->
+    measure conf <= delta ->
+    measure (round delta ffgatherR2 (Stream.hd d) conf) = 0.
+Proof.
+intros [da d] conf delta Hdelta HFS Hlt.
+unfold measure.
+remember (Spect.M.elements (!! conf)) as elems.
+set (C := wbarycenter (map (fun xn => (fst xn, INR (snd xn))) elems)).
+remember (Spect.M.elements (!! (round delta ffgatherR2 da conf))) as nxt_elems.
+assert (Hantec: forall KP, In KP nxt_elems ->
+                  exists Pid, In (Config.loc (conf Pid)) elems /\ R2.eq (round delta ffgatherR2 da conf Pid) KP).
+{ intros KP HinKP.
+  rewrite Heqnxt_elems in HinKP.
+  apply (In_InA R2.eq_equiv) in HinKP.
+  rewrite Spect.M.elements_spec1 in HinKP.
+  generalize (Spect.from_config_spec (round delta ffgatherR2 da conf)).
+  intro Hok. unfold Spect.is_ok in Hok.
+  rewrite Hok in HinKP. clear Hok.
+  destruct HinKP as (Pid, HPid).
+  exists Pid.
+  split; [|now rewrite HPid].
+  generalize (Spect.from_config_spec conf).
+  intro Hok. unfold Spect.is_ok in Hok.
+  destruct (Hok (Config.loc (conf Pid))) as [_ Hex].
+  apply InA_Leibniz.
+  rewrite Heqelems.
+  apply Spect.M.elements_spec1.
+  apply Hex.
+  now exists Pid.
+}
+
+assert (HonlyC: forall KP, In KP nxt_elems -> R2.eq KP C).
+{ intros KP HinKP.
+  destruct (Hantec KP HinKP) as [Pid [HinP HroundP]].
+  rewrite <- HroundP in *. clear HroundP KP.
+  rewrite (round_simplify _ _ _ Pid).
+  destruct (step da Pid) eqn:HeqPact.
+  * destruct p. simpl.
+    rewrite <- Heqelems.
+    unfold Rle_bool.
+    destruct (Rle_dec delta (R2norm (r * (barycenter elems - conf Pid)))).
+    + assert (Hr: 0 <= snd (t, r) <= 1).
+      { apply step_flexibility with da Pid. now symmetry. }
+      simpl in Hr.
+      destruct Hr as [Hr0 Hr1].
+      destruct Hr1 as [Hrlt1 | Hreq1].
+      - exfalso.
+        apply Rlt_irrefl with delta.
+        apply (Rle_lt_trans _ _ _ r0).
+        rewrite R2norm_mul.
+        rewrite (Rabs_pos_eq _ Hr0).
+        rewrite <- R2norm_dist.
+        assert (Hle : R2.dist (barycenter elems) (conf Pid) <= delta).
+        { rewrite R2.dist_sym.
+          apply Rle_trans with (measure conf); trivial; [].
+          apply barycenter_dist_decrease with elems; auto; [|].
+          - rewrite Heqelems, <- Spect.MProp.MP.elements_Empty.
+            intro Hempty. now apply Spect.MProp.MP.empty_is_empty_1, spect_non_nil in Hempty.
+          - intros. unfold measure. apply max_dist_spect_le; now rewrite <- Heqelems. }
+        (* There should be a lemma for this in standard library. *)
+        rewrite <- Rmult_1_l.
+        destruct Hle.
+        -- apply Rmult_le_0_lt_compat; try assumption.
+           apply R2.dist_pos.
+        -- subst delta.
+           apply Rmult_lt_compat_r.
+           now apply Rlt_gt.
+           assumption.
+      - subst r.
+        rewrite R2.mul_1, R2.add_comm, <- R2.add_assoc.
+        pattern (- conf Pid + conf Pid)%R2.
+        rewrite R2.add_comm, R2.add_opp, R2.add_origin.
+        now unfold C.
+    + now unfold C.
+  * unfold FullySynchronous in HFS.
+    inversion HFS.
+    unfold FullySynchronousInstant in H.
+    destruct (H Pid). now symmetry. }
+destruct (max_dist_spect_ex (!! (round delta ffgatherR2 da conf)))
+as [pt0 [pt1 [Hinpt0 [Hinpt1 Hdist]]]].
+apply support_non_nil.
+simpl. rewrite <- Hdist.
+rewrite HonlyC.
+rewrite (HonlyC pt1).
+now apply R2.dist_defined.
+now subst nxt_elems.
+now subst nxt_elems.
+Qed.
+
+Definition lt_config delta x y :=
+  lt (Z.to_nat (up (measure x / delta))) (Z.to_nat (up (measure y / delta))).
+
+Lemma wf_lt_conf (delta: R) (Hdeltapos: delta > 0) : well_founded (lt_config delta).
+Proof.
+  unfold lt_config.
+  apply wf_inverse_image.
+  apply lt_wf.
+Qed.
+
+Lemma lt_config_decrease : forall delta config1 config2, 0 < delta ->
+  measure config1 <= measure config2 - delta -> lt_config delta config1 config2.
+Proof.
+intros delta config1 config2 Hdelta Hle. unfold lt_config.
+rewrite <- Z2Nat.inj_lt.
++ apply Zup_lt. field_simplify; try lra. unfold Rdiv. apply Rmult_le_compat.
+  - apply measure_nonneg.
+  - apply Rlt_le. now apply Rinv_0_lt_compat.
+  - lra.
+  - reflexivity.
++ apply le_IZR. transitivity (measure config1 / delta).
+  - simpl. apply Rdiv_le_0_compat; trivial. apply measure_nonneg.
+  - apply Rlt_le, (proj1 (archimed _)).
++ apply le_IZR. transitivity (measure config2 / delta).
+  - simpl. apply Rdiv_le_0_compat; trivial. apply measure_nonneg.
+  - apply Rlt_le, (proj1 (archimed _)).
+Qed.
+
+(** ***  With the termination, the rest of the proof is easy  **)
+
+Lemma gathered_precise : forall config pt,
+  gathered_at pt config -> forall id, gathered_at (config id) config.
+Proof.
+intros config pt Hgather id id'. transitivity pt.
+- apply Hgather.
+- symmetry. apply (no_byz id), Hgather.
+Qed.
+
+Corollary not_gathered_generalize : forall (config : Config.t) id,
+  ~gathered_at (config id) config -> forall pt, ~gathered_at pt config.
+Proof. intros config id Hnot pt Hgather. apply Hnot. apply (gathered_precise Hgather). Qed.
+
+Lemma not_gathered_exists : forall (config : Config.t) pt,
+  ~ gathered_at pt config -> exists id, ~R2.eq (config id) pt.
+Proof.
+intros config pt Hgather.
+destruct (forallb (fun x => R2dec_bool (config x) pt) Names.names) eqn:Hall.
+- elim Hgather. rewrite forallb_forall in Hall.
+  intro id'. setoid_rewrite R2dec_bool_true_iff in Hall. hnf. repeat rewrite Hall; trivial; apply Names.In_names.
+- rewrite <- negb_true_iff, existsb_forallb, existsb_exists in Hall.
+  destruct Hall as [id' [_ Hid']]. rewrite negb_true_iff, R2dec_bool_false_iff in Hid'. now exists id'.
+Qed.
+
+Lemma gathered_at_forever : forall delta da conf pt,
+  gathered_at pt conf -> gathered_at pt (round delta ffgatherR2 da conf).
+Proof.
+intros delta da conf pt Hgather. rewrite round_simplify.
+intro g.
+assert (Hpt : R2.eq (conf (Good g)) pt) by now rewrite Hgather.
+destruct (step da (Good g)); trivial; [].
+
+assert (Hptinspect: Spect.M.In pt (!! conf)).
+{ unfold Spect.from_config, Spect.M.In.
+  rewrite Spect.multiset_In, Config.list_spec.
+
+  assert (Names.names <> nil).
+  { intro.
+    assert (length Names.names = nG).
+    { rewrite Names.names_length. unfold N.nG, N.nB. omega. }
+      rewrite <- length_zero_iff_nil in H.
+    generalize Hyp_nG. omega.
+  }
+
+  destruct Names.names.
+  - exfalso; now apply H.
+  - revert dependent i. intro id. apply (no_byz id). intros g' **.
+    now apply InA_cons_hd.
+}
+
+assert (Hnotpt_notinspect: forall q, ~ R2.eq q pt -> ~Spect.M.In q (!!conf)).
+{ intros q Hnoteq.
+  unfold Spect.from_config, Spect.M.In.
+  rewrite Spect.multiset_In, Config.list_spec.
+
+  intro HinA.
+  apply Hnoteq.
+  generalize (@InA_map_iff Names.ident R2.t Logic.eq R2.eq).
+  intro HInMapIff.
+  rewrite map_map, HInMapIff in HinA; autoclass.
+  destruct HinA as [x [Heq Hin]].
+  rewrite <- Heq.
+  apply (no_byz x), Hgather.
+}
+
+assert (Hspect: eqlistA Spect.eq_elt (Spect.elements (!! conf)) ((pt, nG) :: nil)).
+{ apply Preliminary.PermutationA_length1, NoDupA_equivlistA_PermutationA; autoclass.
+  + apply Spect.elements_NoDupA.
+  + repeat constructor. rewrite InA_nil. tauto.
+  + intros [x n]. split; intro Hin.
+    - left. destruct (Spect.elt_dec (x, n) (pt, nG)) as [? | Habs]; auto; [].
+      rewrite Spect.elements_In in Hin.
+      now elim (Hnotpt_notinspect x).
+    - inv Hin; try (rewrite InA_nil in *; tauto); [].
+      rewrite Spect.elements_In. hnf in *; simpl in *. now subst. }
+
+assert (HnG := Spect.cardinal_from_config conf).
+rewrite Spect.cardinal_fold_elements in HnG.
+unfold N.nG, N.nB in HnG.
+
+destruct (Spect.elements (!! conf)) as [| [pt' n] [| ]].
++ simpl in HnG. generalize Hyp_nG. omega.
++ inv Hspect. hnf in *; simpl in *; subst.
+  assert (n = nG) by omega. subst n. clear HnG.
+  destruct p.
+  unfold wbarycenter. simpl.
+  rewrite Rplus_0_r, 3 R2.add_origin.
+  rewrite 3 R2.mul_morph.
+  assert (HnG := Hyp_nG). apply le_INR in HnG. simpl in HnG.
+  replace (1 / INR nG * INR nG) with 1%R by (field; lra). rewrite 3 R2.mul_1.
+  rewrite 2 R2.add_opp, 2 R2.mul_origin, R2.add_origin.
+  now destruct_match.
++ repeat match goal with H : eqlistA _ _ _ |- _ => inv H end.
+Qed.
+
+Lemma gathered_at_OK : forall delta d conf pt, gathered_at pt conf -> Gather pt (execute delta ffgatherR2 d conf).
+Proof.
+cofix Hind. intros delta d conf pt Hgather. constructor.
++ clear Hind. simpl. assumption.
++ rewrite execute_tail. apply Hind. now apply gathered_at_forever.
+Qed.
+
+
+Lemma not_barycenter_moves:
+  forall delta d (config : Config.t) gid,
+    delta > 0 ->
+    FullySynchronous d ->
+    ~R2.eq (config gid) (wbarycenter (map (fun xn => (fst xn, INR (snd xn))) (Spect.M.elements (!! config)))) ->
+    ~R2.eq (round delta ffgatherR2 (Stream.hd d) config gid) (config gid).
+Proof.
+  intros delta d config gid Hdelta HFSync Hnotbary Hnotmove.
+  apply Hnotbary. clear Hnotbary.
+  rewrite (round_simplify _ _ _ gid) in Hnotmove.
+  remember (step (Stream.hd d) gid) as Pact.
+  destruct Pact.
+  * destruct p. simpl in Hnotmove.
+    remember (Spect.M.elements (!! config)) as elems.
+    unfold Rle_bool in Hnotmove.
+    destruct (Rle_dec delta (R2norm (r * (wbarycenter
+                         (map (fun xn : Spect.M.elt * nat => (fst xn, INR (snd xn)))
+                            elems) - config gid)))).
+    + rewrite <- R2.add_origin with (u := config gid) in Hnotmove at 3.
+      apply R2.add_reg_l in Hnotmove.
+      apply R2.mul_integral in Hnotmove.
+      destruct Hnotmove as [Hr0 | Heq].
+      - exfalso.
+        subst r.
+        rewrite R2norm_mul, Rabs_R0, Rmult_0_l in r0.
+        apply Rlt_irrefl with delta.
+        now apply (Rle_lt_trans _ _ _ r0).
+      - now rewrite R2sub_origin in Heq.
+    + now symmetry.
+  * unfold FullySynchronous in HFSync.
+    unfold FullySynchronousInstant in HFSync.
+    destruct d.
+    simpl in HeqPact.
+    destruct HFSync.
+    destruct (H gid).
+    simpl.
+    now symmetry.
+Qed.
+
+(** The final theorem. *)
+Theorem FSGathering_in_R2 :
+  forall delta d, delta > 0 -> FullySynchronous d -> FullSolGathering ffgatherR2 d delta.
+Proof.
+intros delta d Hdelta HFS conf. revert d HFS. pattern conf.
+apply (well_founded_ind (wf_lt_conf Hdelta)). clear conf.
+intros conf Hind [da d] HFS.
+(* Are we already gathered? *)
+destruct (gathered_at_dec conf (conf (Good g1))) as [Hmove | Hmove];
+[| destruct (gathered_at_dec (round delta ffgatherR2 da conf)
+                             (round delta ffgatherR2 da conf (Good g1))) as [Hmove' | Hmove']].
+* (* If we are already gathered, not much to do *)
+  exists (conf (Good g1)). now apply Stream.Now, gathered_at_OK.
+* (* If we are gathered at the next step, not much to do either. *)
+  exists (round delta ffgatherR2 da conf (Good g1)).
+ apply Stream.Later, Stream.Now. rewrite execute_tail. now apply gathered_at_OK.
+* (* General case, use [round_lt_config] *)
+  assert (delta <= measure conf).
+  { apply Rnot_lt_le. intro Habs. eapply Rlt_le, round_last_step in Habs; eauto; [].
+    rewrite gathered_measure in Habs. destruct Habs as [pt Habs]. simpl in Habs.
+    apply Hmove'. apply (gathered_precise Habs (Good g1)). }
+  destruct (Hind (round delta ffgatherR2 da conf)) with d as [pt Hpt].
+  + apply lt_config_decrease; trivial; [].
+    change da with (Stream.hd (Stream.cons da d)).
+    now apply round_lt_config.
+  + now destruct HFS.
+  + exists pt. apply Stream.Later. apply Hpt.
+Qed.
+
+Print Assumptions FSGathering_in_R2.
+
+End GatheringinR2.
